TM.computes and loop

Cslib/Computability/Machines/MultiTapeTuring/AddRoutine.lean
@@ -32,6 +32,89 @@ variable {k : ℕ}
 -- b
 -- 0
 
+def isZero (i : Fin k.succ) := ite i (pop i <;> push i []) (pop i <;> push i [OneTwo.one])
+
+@[simp, grind =]
+theorem isZero_eval_list {k : ℕ} {i : Fin k.succ} {tapes : Fin k.succ → List (List OneTwo)}
+  {h_tapes_i : tapes i ≠ []} :
+  (isZero i).eval_list tapes = .some (Function.update tapes i (
+    (if (tapes i).head h_tapes_i = [] then [OneTwo.one] else []) :: (tapes i).tail)) := by
+  simp [isZero, ite_eval, h_tapes_i]
+  grind
+
+public def neq {k : ℕ} (q s t : Fin k.succ)
+  (h_neq : q ≠ s := by decide) (h_neq' : q ≠ t := by decide) (h_neq'' : s ≠ t := by decide) :
+  MultiTapeTM k.succ (WithSep OneTwo) :=
+  (eq q s t h_neq h_neq' h_neq'') <;> (isZero ⟨t, by omega⟩)
+
+@[simp, grind =]
+public theorem neq_eval_list {k : ℕ} {q s t : Fin k.succ}
+  {h_neq : q ≠ s} {h_neq' : q ≠ t} {h_neq'' : s ≠ t}
+  {tapes : Fin k.succ → List (List OneTwo)}
+  {h_q_nonempty : tapes q ≠ []} {h_s_nonempty : tapes s ≠ []} :
+  (eq q s t (h_neq := h_neq) (h_neq' := h_neq') (h_neq'' := h_neq'')).eval_list tapes =
+    Part.some (Function.update tapes t
+      ((if (tapes q).head h_q_nonempty = (tapes s).head h_s_nonempty then
+        []
+      else
+        [.one]) :: (tapes t))) := by
+  sorry
+
+/-- Execute `tm` a number of times as given by the first word on tape `i`.
+Note that the iteration counter is not directly available to the TM. -/
+def loop (i : Fin k) (tm : MultiTapeTM k (WithSep OneTwo)) :
+    MultiTapeTM (k + 3) (WithSep OneTwo) :=
+  let target : Fin (k + 3) := ⟨k, by omega⟩
+  let counter : Fin (k + 3) := ⟨k.succ, by omega⟩
+  let cond : Fin (k + 3) := ⟨k.succ.succ, by omega⟩
+  copy ⟨i, by omega⟩ target (h_neq := by grind) <;>
+  push counter [] <;>
+  neq target counter cond (by grind) (by grind) (by grind) <;>
+  doWhile cond (
+    pop cond <;>
+    tm.extend (by omega) <;>
+    succ counter <;>
+    neq target counter cond (by grind) (by grind) (by grind)) <;>
+  pop cond <;>
+  pop counter <;>
+  pop target
+
+theorem loop_eval_list_inner {i : Fin k}
+  {tm : MultiTapeTM k (WithSep OneTwo)}
+  {f_tm : (Fin k → List (List OneTwo)) → (Fin k → List (List OneTwo))}
+  {tapes : Fin (k + 3) → List (List OneTwo)}
+  {h_tapes_i : tapes ⟨i, by omega⟩ ≠ []} :
+  let target : Fin (k + 3) := ⟨k, by omega⟩
+  let counter : Fin (k + 3) := ⟨k.succ, by omega⟩
+  let cond : Fin (k + 3) := ⟨k.succ.succ, by omega⟩
+  (pop cond <;>
+    tm.extend (by omega) <;>
+    succ counter <;>
+    neq target counter cond (by grind) (by grind) (by grind)).eval_list tapes = do
+    let tapes := (tm.extend (by omega)).eval_list tapes
+    Function.update tapes counter (
+      (dya ((dya_inv ((tapes ⟨i, by omega⟩).head h_tapes_i)).succ)) :: (tapes counter).tail) := by
+    tm.eva
+  (loop i tm).eval_list tapes = .some
+    fun j => if h : j < k then
+      (f_tm^[dya_inv ((tapes ⟨i, by omega⟩).head h_tapes_i)] (fun i => tapes ⟨i, by omega⟩)) ⟨j, h⟩
+    else
+      tapes j := by
+  sorry
+
+theorem loop_eval_list {i : Fin k}
+  {tm : MultiTapeTM k (WithSep OneTwo)}
+  {f_tm : (Fin k → List (List OneTwo)) → (Fin k → List (List OneTwo))}
+  {tapes : Fin (k + 3) → List (List OneTwo)}
+  {h_tapes_i : tapes ⟨i, by omega⟩ ≠ []} :
+  (loop i tm).eval_list tapes = .some
+    fun j => if h : j < k then
+      (f_tm^[dya_inv ((tapes ⟨i, by omega⟩).head h_tapes_i)] (fun i => tapes ⟨i, by omega⟩)) ⟨j, h⟩
+    else
+      tapes j := by
+  sorry
+
+/-- Execute `tm` in a loop as long as running `cond` pushes a non-empty value to the last tape. -/
 def whileCond (cond : MultiTapeTM k.succ (WithSep α)) (tm : MultiTapeTM k (WithSep α)) :
     MultiTapeTM k.succ (WithSep α) :=
   let k := ⟨k, by omega⟩
@@ -39,15 +122,23 @@ def whileCond (cond : MultiTapeTM k.succ (WithSep α)) (tm : MultiTapeTM k (With
   doWhile k ((pop k) <;> (tm.extend (by omega) <;> cond)) <;>
   (pop ⟨k, by omega⟩)
 
-def not (i : Fin k.succ) := ite i (pop i <;> push i []) (pop i <;> push i [OneTwo.one])
-
-@[simp, grind =]
-theorem not_eval_list {i : Fin k.succ} {tapes : Fin k.succ → List (List OneTwo)}
-  {h_tapes_i : tapes i ≠ []} :
-  (not i).eval_list tapes = .some (Function.update tapes i (
-    (if (tapes i).head h_tapes_i = [] then [OneTwo.one] else []) :: (tapes i).tail)) := by
-  simp [not, ite_eval, h_tapes_i]
+lemma whileCond_eval_list {cond : MultiTapeTM k.succ (WithSep α)}
+  {tm : MultiTapeTM k (WithSep α)}
+  {tm_f : Fin k.succ → List (List α) → Option (Fin k.succ → List (List α))}
+  {cond_f : (Fin k.succ → List (List α)) → List α}
+  {h_cond_f : ∀ t, cond.eval_list t = Part.some (Function.update t ⟨k, _⟩ ((cond_f t) :: (t ⟨k, _⟩)))}
+  {tapes : Fin k.succ → List (List α)}
+  {h_nonempty : tapes ⟨k, by omega⟩ ≠ []} :
+  (whileCond cond tm).eval_list tapes =
+    cond.eval_list tapes >>= fun tapes' =>
+      doWhile_eval_list ⟨k, by omega⟩
+        (Function.update tapes' ⟨k, by omega⟩ (tapes' ⟨k, by omega⟩.tail))
+        (pop ⟨k, by omega⟩)
+        (tm.extend (by omega) <;> cond) >>= fun tapes'' =>
+          pop.eval_list tapes'' := by
+  simp [whileCond, seq_eval_list, doWhile_eval_list, pop_eval_list]
   grind
+
 
 -- public def add₀ : MultiTapeTM 4 (WithSep OneTwo) :=
 --   copy 1 2 <;> push 1 []
@@ -63,15 +154,22 @@ theorem not_eval_list {i : Fin k.succ} {tapes : Fin k.succ → List (List OneTwo
 public def add₀ : MultiTapeTM 4 (WithSep OneTwo) :=
   (((copy 1 2 <;> push 1 []) <;>
   -- Here we have [a, 0 :: b, b]
-  (whileCond ((eq 0 1 3) <;> not 3) (succ 1 <;> succ 2))) <;>
+  (whileCond ((eq 0 1 3) <;> isZero 3) (succ 1 <;> succ 2))) <;>
   -- Here we have [a, a :: b, a + b]
   (pop 1))
+
+-- lemma add₀_while_eval_list {tapes : Fin 4 → List (List OneTwo)}
+--   {h_nonempty₀ : tapes 0 ≠ []} {h_nonempty₁ : tapes 1 ≠ []} :
+--   (whileCond ((eq 0 1 3) <;> not 3) (succ 1 <;> succ 2)).eval_list tapes = .some
+--     (Function.update tapes 2 ((dya (dya_inv ((tapes 0).head h_nonempty₀) +
+--       dya_inv ((tapes 1).head h_nonempty₁)) :: (tapes 2)))) := by
 
 @[simp, grind =]
 theorem add₀_eval_list {tapes : Fin 4 → List (List OneTwo)}
   {h_nonempty₀ : tapes 0 ≠ []} {h_nonempty₁ : tapes 1 ≠ []} :
   add₀.eval_list tapes = .some
-    (Function.update tapes 2 ((dya (dya_inv ((tapes 0).head h_nonempty₀) + dya_inv ((tapes 1).head h_nonempty₁)) :: (tapes 2)))) := by
+    (Function.update tapes 2 ((dya (dya_inv ((tapes 0).head h_nonempty₀) +
+      dya_inv ((tapes 1).head h_nonempty₁)) :: (tapes 2)))) := by
   sorry
 
 -- --- Repeatedly run a sub routine as long as a condition on the symbol
